Added PtrnListFunc.v

Charge!/src/Charge/ModularFunc/ListFunc.v
@@ -1,7 +1,3 @@
-Add Rec LoadPath "/Users/jebe/git/coq-ext-lib/theories" as ExtLib.
-Add Rec LoadPath "/Users/jebe/git/mirror-core/theories" as MirrorCore.
-Add Rec LoadPath "/Users/jebe/git/Charge/Charge!/bin/Charge" as Charge.
-
 Require Import ExtLib.Core.RelDec.
 Require Import ExtLib.Data.Fun.
 Require Import ExtLib.Data.Map.FMapPositive.
@@ -16,7 +12,7 @@ Require Import MirrorCore.syms.SymSum.
 Require Import MirrorCore.Lambda.Expr.
 
 Require Import Charge.Logics.ILogic.
-Require Import Charge.ModularFunc.Nat.
+Require Import Charge.ModularFunc.NatFunc.
 Require Import Charge.ModularFunc.Prop.
 Require Import Charge.ModularFunc.Denotation.
 
@@ -30,23 +26,11 @@ Set Maximal Implicit Insertion.
 
 Inductive list_func (typ : Type) :=
   | pNil : typ -> list_func typ
-  | pCons : typ -> list_func typ
-  | pLength : typ -> list_func typ
-  | pNoDup : typ -> list_func typ
-  | pIn : typ -> list_func typ
-  | pMap : typ -> typ -> list_func typ
-  | pFold : typ -> typ -> list_func typ
-  | pZip : typ -> typ -> list_func typ.
+  | pCons : typ -> list_func typ.
 
 Class ListFunc (typ func : Type) := {
   fNil  : typ -> func;
   fCons : typ -> func;
-  fLength : typ -> func;
-  fNoDup : typ -> func;
-  fIn : typ -> func;
-  fMap : typ -> typ -> func;
-  fFold : typ -> typ -> func;
-  fZip : typ -> typ -> func;
   
   listS : func -> option (list_func typ)
 }.
@@ -59,12 +43,6 @@ Section ListFuncSum.
 	  ListFunc typ (OneOf m) := {
 	    fNil t := Into (fNil t) p pf;
 	    fCons t := Into (fCons t) p pf;
-	    fLength t := Into (fLength t) p pf;
-	    fNoDup t := Into (fNoDup t) p pf;
-	    fIn t := Into (fIn t) p pf;
-	    fMap t u := Into (fMap t u) p pf;
-	    fFold t u := Into (fFold t u) p pf;
-	    fZip t u := Into (fZip t u) p pf;
 	    
 	    listS f :=
 	      match f with
@@ -82,12 +60,6 @@ Section ListFuncSum.
     	ListFunc typ (expr typ func) := {
     	  fNil t := Inj (fNil t);
     	  fCons t := Inj (fCons t);
-    	  fLength t := Inj (fLength t);
-    	  fNoDup t := Inj (fNoDup t);
-    	  fIn t := Inj (fIn t);
-    	  fMap t1 t2 := Inj (fMap t1 t2);
-    	  fFold t1 t2 := Inj (fFold t1 t2);
-    	  fZip t1 t2 := Inj (fZip t1 t2);
          
           listS f := match f with
           			   | Inj f => listS f
@@ -103,29 +75,15 @@ Section ListFuncInst.
   Context {Heq : RelDec (@eq typ)} {HC : RelDec_Correct Heq}.
   
   Context {Typ2_tyArr : Typ2 _ Fun}.
-  Context {Typ2_tyProd : Typ2 _ prod}.
   Context {Typ1_tyList : Typ1 _ list}.
-  Context {Typ0_tyProp : Typ0 _ Prop}.
-  Context {Typ0_tyNat : Typ0 _ nat}.
-  
-  Context {Typ0_tyPropOk : Typ0Ok Typ0_tyProp}.
   
   Let tyArr : typ -> typ -> typ := @typ2 _ _ _ Typ2_tyArr.
-  Let tyProd : typ -> typ -> typ := @typ2 _ _ _ Typ2_tyProd.
   Let tyList : typ -> typ := @typ1 _ _ _ _.
-  Let tyProp : typ := @typ0 _ _ _ Typ0_tyProp.
-  Let tyNat : typ := @typ0 _ _ _ Typ0_tyNat.
 
   Global Instance ListFuncInst : ListFunc typ (list_func typ) := 
     {
       fNil := pNil;
       fCons := pCons;
-      fLength := pLength;
-      fNoDup := pNoDup;
-      fIn := pIn;
-      fMap := pMap;
-      fFold := pFold;
-      fZip := pZip;
       
       listS f := Some f
     }.
@@ -134,27 +92,12 @@ Section ListFuncInst.
     match lf with
       | pNil t => Some (tyList t)
       | pCons t => Some (tyArr t (tyArr (tyList t) (tyList t)))
-      | pLength t => Some (tyArr (tyList t) tyNat)
-      | pNoDup t => Some (tyArr (tyList t) tyProp)
-      | pIn t => Some (tyArr t (tyArr (tyList t) tyProp))
-      | pMap t1 t2 => Some (tyArr (tyArr t1 t2) (tyArr (tyList t1) (tyList t2)))
-      | pFold t1 t2 => Some (tyArr (tyArr t2 (tyArr t1 t1)) (tyArr t1 (tyArr (tyList t2) t1))) 
-      | pZip t1 t2 => Some (tyArr (tyList t1) (tyArr (tyList t2) (tyList (tyProd t1 t2))))
     end.
 
   Definition list_func_eq (a b : list_func typ) : option bool :=
     match a , b with
       | pNil t1, pNil t2 => Some (t1 ?[ eq ] t2)
       | pCons t1, pCons t2 => Some (t1 ?[ eq ] t2)
-      | pLength t1, pLength t2 => Some (t1 ?[ eq ] t2)
-      | pNoDup t1, pNoDup t2 => Some (t1 ?[ eq ] t2)
-      | pIn t1, pIn t2 => Some (t1 ?[ eq ] t2)
-      | pMap t1 t2, pMap t3 t4 => Some (t1 ?[ eq ] t3 &&
-	      				   t2 ?[ eq ] t4)%bool
-      | pFold t1 t2, pFold t3 t4 => Some (t1 ?[ eq ] t3 &&
-	      				     t2 ?[ eq ] t4)%bool
-      | pZip t1 t2, pZip t3 t4 => Some (t1 ?[ eq ] t3 &&
-	      				   t2 ?[ eq ] t4)%bool
       | _, _ => None
     end.
 
@@ -207,28 +150,6 @@ Section ListFuncInst.
   Definition consD t : typD (tyArr t (tyArr (tyList t) (tyList t))) :=
     tyArrR2 (fun (x : typD t) (xs : typD (tyList t)) =>
                listR (cons x (trmD xs (listE eq_refl)))).
-  
-  Definition lengthD t := tyArrR (fun (xs : typD (tyList t)) => 
-    natR (List.length (listD xs))).
-  
-  Definition NoDupD t := 
-    tyArrR (fun (xs : typD (tyList t)) => PropR (NoDup (listD xs))).
-  
-  Definition InD t := 
-    tyArrR2 (fun (x : typD t) (xs : typD (tyList t)) => 
-      PropR (In x (listD xs))).
-
-  Definition mapD t u :=
-    tyArrR2 (fun (f : typD (tyArr t u)) (xs : typD (tyList t)) => 
-      (listR (map (tyArrD f) (listD xs)))).
-
-  Definition foldD t u :=
-    tyArrR3 (fun (f : typD (tyArr u (tyArr t t))) (acc : typD t) (lst : typD (tyList u)) =>
-      fold_right (tyArrD2 f) acc (listD lst)).
-
-  Definition zipD t u :=
-    tyArrR2 (fun (xs : typD (tyList t)) (ys : typD (tyList u)) =>
-      trmR (combine (listD xs) (listD ys)) (listE (pairE (t := t) (u := u) eq_refl eq_refl))).
 
   Lemma listD_nil t : listD (nilD t) = nil.
   Proof.
@@ -240,117 +161,46 @@ Section ListFuncInst.
     reflexivity.
   Qed.
 
-	 Definition list_func_symD lf :=
-		match lf as lf return match typeof_list_func lf return Type with
-								| Some t => typD t
-								| None => unit
-							  end with
-	    | pNil t => nilD t
-	    | pCons t => consD t
-	    | pLength t => lengthD t
-	    | pNoDup t => NoDupD t
-	    | pIn t => InD t
-	    | pMap t1 t2 => mapD t1 t2
-	    | pFold t1 t2 => foldD t1 t2
-	    | pZip t1 t2 => zipD t1 t2
-	 end.
+  Definition list_func_symD lf :=
+    match lf as lf return match typeof_list_func lf return Type with
+			    | Some t => typD t
+			    | None => unit
+			  end with
+      | pNil t => nilD t
+      | pCons t => consD t
+    end.
 
-	Global Instance RSym_ListFunc : SymI.RSym (list_func typ) := {
-	  typeof_sym := typeof_list_func;
-	  symD := list_func_symD;
-	  sym_eqb := list_func_eq
-	}.
+  Global Instance RSym_ListFunc : SymI.RSym (list_func typ) := 
+    {
+      typeof_sym := typeof_list_func;
+      symD := list_func_symD;
+      sym_eqb := list_func_eq
+    }.
 
-	Global Instance RSymOk_ListFunc : SymI.RSymOk RSym_ListFunc.
-	Proof.
-		split; intros.
-		destruct a, b; simpl; try apply I.
-		+ consider (t ?[ eq ] t0); intuition congruence.
-		+ consider (t ?[ eq ] t0); intuition congruence.
-		+ consider (t ?[ eq ] t0); intuition congruence.
-		+ consider (t ?[ eq ] t0); intuition congruence.
-		+ consider (t ?[ eq ] t0); intuition congruence.
-		+ consider (t ?[ eq ] t1 && t0 ?[ eq ] t2)%bool; intuition congruence. 
-		+ consider (t ?[ eq ] t1 && t0 ?[ eq ] t2)%bool; intuition congruence. 
-		+ consider (t ?[ eq ] t1 && t0 ?[ eq ] t2)%bool; intuition congruence. 
-	Qed.
+  Global Instance RSymOk_ListFunc : SymI.RSymOk RSym_ListFunc.
+  Proof.
+    split; intros.
+    destruct a, b; simpl; try apply I.
+    + consider (t ?[ eq ] t0); intuition congruence.
+    + consider (t ?[ eq ] t0); intuition congruence.
+  Qed.
 
 End ListFuncInst.
 
 Section MakeList.
-	Context {typ func : Type} {H : ListFunc typ func}.
-
-	Definition mkNil t : expr typ func := Inj (fNil t).
-	Definition mkCons (t : typ) (x xs : expr typ func) := App (App (fCons t) x) xs.
-	Definition mkLength (t : typ) (lst : expr typ func) := App (fLength t) lst.
-	Definition mkNoDup (t : typ) (lst : expr typ func) := App (fNoDup t) lst.
-	Definition mkIn (t : typ) (x lst : expr typ func) := App (App (fIn t) x) lst.
-	Definition mkMap (t u : typ) (f lst : expr typ func) :=  App (App (fMap t u) f) lst.
-	Definition mkFold (t u : typ) (f acc lst : expr typ func) :=  App (App (App (fFold t u) f) acc) lst.
-	Definition mkZip (t u : typ) (xs ys : expr typ func) := App (App (fZip t u) xs) ys.
-	
+  Context {typ func : Type} {H : ListFunc typ func}.
+  
+  Definition mkNil t : expr typ func := Inj (fNil t).
+  Definition mkCons (t : typ) (x xs : expr typ func) := App (App (fCons t) x) xs.
+  
 End MakeList.
-
-Section ListOps.
-  Context {typ func : Type} {RType_typ : RType typ}.
-  Context {BF: BaseFunc typ func} {LF : ListFunc typ func}.
-  Context {RSym_func : RSym func}.
-  Context {LT : ListType typ}.
- 
-  Context {Typ2_tyArr : Typ2 _ Fun}.
-(*
-  Definition list_to_expr (t : typ) (lst : list (typD t)) :=
-    fold_right (fun x acc => mkCons t (mkConst t x) acc) (mkNil t) lst.
- *)
-  Fixpoint expr_to_list (e : expr typ func) : (list (expr typ func) * expr typ func) :=
-    match e with
-      | App (App f x) xs =>
-        match listS f with
-          | Some (pCons t) =>
-            let p := expr_to_list xs in (x::fst p, snd p)
-          | _ => (nil, e)
-        end
-      | _ => (nil, e)
-    end.
-  
-  Lemma expr_to_list_nil (e1 e2 : expr typ func) (H : expr_to_list e1 = (nil, e2)) : e1 = e2.
-  Proof.
-    destruct e1; simpl in *; try (solve [inversion H; reflexivity]).
-    destruct e1_1; simpl in *; try (solve [inversion H; reflexivity]).
-    destruct e1_1_1; simpl in *; try (solve [inversion H; reflexivity]).
-    destruct (listS f); simpl in *; try (solve [inversion H; reflexivity]).
-    destruct l; simpl in *; try (solve [inversion H; reflexivity]).
-  Qed.
-
-  Lemma expr_to_list_cons tus tvs t (e1 e2 : expr typ func) x xs (H : expr_to_list e1 = (x::xs, e2))
-    (Htype : typeof_expr tus tvs e1 = Some (tyList t)) :
-    exists e3, expr_to_list e3 = (xs, e2) /\ e1 = mkCons t x e3.
-  Proof.
-    destruct e1; simpl in *; try (solve [inversion H; reflexivity]).
-    destruct e1_1; simpl in *; try (solve [inversion H; reflexivity]).
-    destruct e1_1_1; simpl in *; try (solve [inversion H; reflexivity]).
-    remember (listS f); destruct o; simpl in *; try (solve [inversion H; reflexivity]).
-    destruct l; simpl in *; try (solve [inversion H; reflexivity]).
-    inversion H; subst.
-    exists e1_2.
-    split.
-    destruct (expr_to_list e1_2). reflexivity.
-    unfold mkCons.
-    symmetry in Heqo.
-(*    forward.*)
-	admit.
-  Admitted.
-  
-End ListOps.
 
 Section ListFuncOk.
   Context {typ func : Type} {RType_typ : RType typ}.
   Context {LF: ListFunc typ func} {RSym_func : RSym func}.
   Context {RelDec_eq : RelDec (@eq typ)}.
-  Context {BT : BaseType typ} {BTD : BaseTypeD BT}.
-  Context {LT : ListType typ} {LTD : ListTypeD LT}.
   Context {Typ2_tyArr : Typ2 _ Fun}.
-  Context {Typ0_Prop : Typ0 _ Prop}.
+  Context {Typ1_tyList : Typ1 _ list}.
 
   Class ListFuncOk := {
     lf_funcAsOk (f : func) (e : list_func typ) : listS f = Some e -> 
@@ -358,44 +208,27 @@ Section ListFuncOk.
         funcAs f t = 
         funcAs (RSym_func := RSym_ListFunc) e t;
     lf_fNilOk t : listS (fNil t) = Some (pNil t);
-    lf_fConsOk t : listS (fCons t) = Some (pCons t);
-    lf_fLengthOk t : listS (fLength t) = Some (pLength t);
-    lf_fNoDupOk t : listS (fNoDup t) = Some (pNoDup t);
-    lf_fInOk t : listS (fIn t) = Some (pIn t);
-    lf_fMapOk t u : listS (fMap t u) = Some (pMap t u);
-    lf_fFoldOk t u : listS (fFold t u) = Some (pFold t u);
-    lf_fZipOk t u : listS (fZip t u) = Some (pZip t u)
+    lf_fConsOk t : listS (fCons t) = Some (pCons t)
   }.
 
 End ListFuncOk.
 
-Implicit Arguments ListFuncOk [[LF] [RType_typ] [RSym_func] [RelDec_eq] [LT] [LTD]
-                               [Typ2_tyArr] [Typ0_Prop] [BT] [BTD]].
+Implicit Arguments ListFuncOk [[LF] [RType_typ] [RSym_func] [RelDec_eq]
+                               [Typ2_tyArr] [Typ1_tyList]].
                                
 Section ListFuncBaseOk.
   Context {typ func : Type} {RType_typ : RType typ}.
   Context {LF: ListFunc typ func} {RSym_func : RSym func}.
   Context {RelDec_eq : RelDec (@eq typ)}.
   Context {RelDec_eqOk : RelDec_Correct RelDec_eq}.
-  Context {BT : BaseType typ} {BTD : BaseTypeD BT}.
-  Context {LT : ListType typ} {LTD : ListTypeD LT}.
 
   Context {Typ2_tyArr : Typ2 _ Fun}.
-  Context {Typ0_Prop : Typ0 _ Prop}.
-
-  Let tyArr : typ -> typ -> typ := @typ2 _ _ _ _.
+  Context {Typ1_tyList : Typ1 _ list}.
   
   Global Program Instance ListFuncBaseOk : 
   	ListFuncOk typ (RSym_func := RSym_ListFunc) (list_func typ) := {
     lf_funcAsOk := fun _ _ _ _ => eq_refl;
-    lf_fNilOk t := eq_refl;
-    lf_fConsOk t := eq_refl;
-    lf_fLengthOk t := eq_refl;
-    lf_fNoDupOk t := eq_refl;
-    lf_fInOk t := eq_refl;
-    lf_fMapOk t u := eq_refl;
-    lf_fFoldOk t u := eq_refl;
-    lf_fZipOk t u := eq_refl
+    lf_fNilOk t := eq_refl
   }.
 
 End ListFuncBaseOk.
@@ -405,11 +238,12 @@ Section ListFuncExprOk.
   Context {HROk : RTypeOk}.
   Context {A : Type} {RSymA : RSym A}.
   Context {Typ2Ok_tyArr : Typ2Ok Typ2_tyArr}.
+  Context {Typ1Ok_tyList : Typ1Ok Typ1_tyList}.
   Context {RSym_funcOk : RSymOk RSym_func0}.
   
 
   Let tyArr : typ -> typ -> typ := @typ2 _ _ _ _.
-  Let tyProp : typ := @typ0 _ _ _ _.
+  Let tyList : typ -> typ  := @typ1 _ _ _ _.
 
   Lemma ListFunc_typeOk (f : func) (e : list_func typ) (H : listS f = Some e) :
     typeof_sym f = typeof_list_func e.
@@ -433,7 +267,7 @@ Section ListFuncExprOk.
   Proof.
     rewrite (lf_funcAsOk _ H1) in H2.
     unfold funcAs in H2; simpl in *.
-    forward.
+    forward. rewrite <- r. reflexivity.
   Qed.
 
   Lemma lf_nil_type_eq tus tvs (e : expr typ func) t t' df
@@ -442,6 +276,16 @@ Section ListFuncExprOk.
   Proof.
     destruct e; simpl in *; try congruence.
     autorewrite with exprD_rw in H2; simpl in H2; forward; inv_all; subst.
+    eapply lf_nil_func_type_eq; eassumption.
+  Qed.
+
+  Lemma list_nil_type_eq (f : func) (t u : typ) 
+        (H1 : listS f = Some (pNil t)) (H2 : typeof_sym f = Some u) :
+    u = tyList t.
+  Proof.
+    destruct (ExprFacts.typeof_expr_exprD' _ _ _ nil nil (Inj f) H2) as [x H].
+    autorewrite with exprD_rw in H.
+    simpl in H. forward.
     eapply lf_nil_func_type_eq; eassumption.
   Qed.
 
@@ -464,162 +308,14 @@ Section ListFuncExprOk.
     eapply lf_cons_func_type_eq; eassumption.
   Qed.
 
-  Lemma lf_length_func_type_eq (f : func) t t' df
-    (H1 : listS f = Some (pLength t)) (H2 : funcAs f t' = Some df) :
-    t' = tyArr (tyList t) tyNat.
+  Lemma list_cons_type_eq (f : func) (t u : typ) 
+        (H1 : listS f = Some (pCons t)) (H2 : typeof_sym f = Some u) :
+    u = tyArr t (tyArr (tyList t) (tyList t)).
   Proof.
-    rewrite (lf_funcAsOk _ H1) in H2.
-    unfold funcAs in H2; simpl in *.
-    forward.
-    rewrite <- r. reflexivity.
-  Qed.
-
-  Lemma lf_length_type_eq tus tvs (e : expr typ func) t t' df
-    (H1 : listS e = Some (pLength t)) (H2 : exprD' tus tvs t' e = Some df) :
-    t' = tyArr (tyList t) tyNat.
-  Proof.
-    destruct e; simpl in *; try congruence.
-    autorewrite with exprD_rw in H2; simpl in H2; forward; inv_all; subst.
-    eapply lf_length_func_type_eq; eassumption.
-  Qed.
-
-  Lemma lf_NoDup_func_type_eq (f : func) t t' df
-    (H1 : listS f = Some (pNoDup t)) (H2 : funcAs f t' = Some df) :
-    t' = tyArr (tyList t) tyProp.
-  Proof.
-    rewrite (lf_funcAsOk _ H1) in H2.
-    unfold funcAs in H2; simpl in *.
-    forward.
-    rewrite <- r. reflexivity.
-  Qed.
-
-  Lemma lf_NoDup_type_eq tus tvs (e : expr typ func) t t' df
-    (H1 : listS e = Some (pNoDup t)) (H2 : exprD' tus tvs t' e = Some df) :
-    t' = tyArr (tyList t) tyProp.
-  Proof.
-    destruct e; simpl in *; try congruence.
-    autorewrite with exprD_rw in H2; simpl in H2; forward; inv_all; subst.
-    eapply lf_NoDup_func_type_eq; eassumption.
-  Qed.
-
-  Lemma lf_In_func_type_eq (f : func) t t' df
-    (H1 : listS f = Some (pIn t)) (H2 : funcAs f t' = Some df) :
-    t' = tyArr t (tyArr (tyList t) tyProp).
-  Proof.
-    rewrite (lf_funcAsOk _ H1) in H2.
-    unfold funcAs in H2; simpl in *.
-    forward.
-    rewrite <- r. reflexivity.
-  Qed.
-
-  Lemma lf_In_type_eq tus tvs (e : expr typ func) t t' df
-    (H1 : listS e = Some (pIn t)) (H2 : exprD' tus tvs t' e = Some df) :
-    t' = tyArr t (tyArr (tyList t) tyProp).
-  Proof.
-    destruct e; simpl in *; try congruence.
-    autorewrite with exprD_rw in H2; simpl in H2; forward; inv_all; subst.
-    eapply lf_In_func_type_eq; eassumption.
-  Qed.
-
-  Lemma lf_map_func_type_eq (f : func) t u t' df
-    (H1 : listS f = Some (pMap t u)) (H2 : funcAs f t' = Some df) :
-    t' = tyArr (tyArr t u) (tyArr (tyList t) (tyList u)).
-  Proof.
-    rewrite (lf_funcAsOk _ H1) in H2.
-    unfold funcAs in H2; simpl in *.
-    forward.
-    rewrite <- r. reflexivity.
-  Qed.
-
-  Lemma lf_map_type_eq tus tvs (e : expr typ func) t u t' df
-    (H1 : listS e = Some (pMap t u)) (H2 : exprD' tus tvs t' e = Some df) :
-    t' = tyArr (tyArr t u) (tyArr (tyList t) (tyList u)).
-  Proof.
-    destruct e; simpl in *; try congruence.
-    autorewrite with exprD_rw in H2; simpl in H2; forward; inv_all; subst.
-    eapply lf_map_func_type_eq; eassumption.
-  Qed.
-
-  Lemma lf_fold_func_type_eq (f : func) t u t' df
-    (H1 : listS f = Some (pFold t u)) (H2 : funcAs f t' = Some df) :
-    t' = tyArr (tyArr u (tyArr t t)) (tyArr t (tyArr (tyList u) t)).
-  Proof.
-    rewrite (lf_funcAsOk _ H1) in H2.
-    unfold funcAs in H2; simpl in *.
-    forward.
-    rewrite <- r. reflexivity.
-  Qed.
-
-  Lemma lf_fold_type_eq (e : expr typ func) tus tvs t u t' df
-    (H1 : listS e = Some (pFold t u)) (H2 : exprD' tus tvs t' e = Some df) :
-    t' = tyArr (tyArr u (tyArr t t)) (tyArr t (tyArr (tyList u) t)).
-  Proof.
-    destruct e; simpl in *; try congruence.
-    autorewrite with exprD_rw in H2; simpl in H2; forward; inv_all; subst.
-    eapply lf_fold_func_type_eq; eassumption.
-  Qed.
-
-  Lemma lf_zip_func_type_eq (f : func) t u t' df
-    (H1 : listS f = Some (pZip t u)) (H2 : funcAs f t' = Some df) :
-    t' = tyArr (tyList t) (tyArr (tyList u) (tyList (tyProd t u))).
-  Proof.
-    rewrite (lf_funcAsOk _ H1) in H2.
-    unfold funcAs in H2; simpl in *.
-    forward.
-    rewrite <- r. reflexivity.
-  Qed.
-
-  Lemma lf_zip_type_eq tus tvs (e : expr typ func) t u t' df
-    (H1 : listS e = Some (pZip t u)) (H2 : exprD' tus tvs t' e = Some df) :
-    t' = tyArr (tyList t) (tyArr (tyList u) (tyList (tyProd t u))).
-  Proof.
-    destruct e; simpl in *; try congruence.
-    autorewrite with exprD_rw in H2; simpl in H2; forward; inv_all; subst.
-    eapply lf_zip_func_type_eq; eassumption.
-  Qed.
-
-  Existing Instance RSym_sum.
-
-  Global Program Instance ListFuncOkSumR : ListFuncOk typ ((A + func)%type) := {
-    lf_funcAsOk := 
-      fun a f H t => 
-        match a with
-          | inl b => _
-          | inr b => _
-        end;
-    lf_fNilOk t := lf_fNilOk (func := func) t;
-    lf_fConsOk t := lf_fConsOk (func := func) t;
-    lf_fLengthOk t := lf_fLengthOk (func := func) t;
-    lf_fNoDupOk t := lf_fNoDupOk (func := func) t;
-    lf_fInOk t := lf_fInOk (func := func) t;
-    lf_fMapOk t u := lf_fMapOk (func := func) t u;
-    lf_fFoldOk t u := lf_fFoldOk (func := func) t u;
-    lf_fZipOk t u := lf_fZipOk (func := func) t u
-  }.
-  Next Obligation.
-    apply (lf_funcAsOk (func := func)).
-    apply H.
-  Qed.
-
-  Global Program Instance ListFuncOkSumL : ListFuncOk typ ((func + A)%type) := {
-    lf_funcAsOk := 
-      fun a f H t => 
-        match a with
-          | inl b => _
-          | inr b => _
-        end;
-    lf_fNilOk t := lf_fNilOk (func := func) t;
-    lf_fConsOk t := lf_fConsOk (func := func) t;
-    lf_fLengthOk t := lf_fLengthOk (func := func) t;
-    lf_fNoDupOk t := lf_fNoDupOk (func := func) t;
-    lf_fInOk t := lf_fInOk (func := func) t;
-    lf_fMapOk t u := lf_fMapOk (func := func) t u;
-    lf_fFoldOk t u := lf_fFoldOk (func := func) t u;
-    lf_fZipOk t u := lf_fZipOk (func := func) t u
-  }.
-  Next Obligation.
-    apply (lf_funcAsOk (func := func)).
-    apply H.
+    destruct (ExprFacts.typeof_expr_exprD' _ _ _ nil nil (Inj f) H2) as [x H].
+    autorewrite with exprD_rw in H.
+    simpl in H. forward.
+    eapply lf_cons_func_type_eq; eassumption.
   Qed.
 
 End ListFuncExprOk.
@@ -630,7 +326,7 @@ Section MakeListFuncSound.
           {RSym_funcOk : RSymOk RSym_func0}.
 
   Let tyArr : typ -> typ -> typ := @typ2 _ _ _ _.
-  Let tyProp : typ := @typ0 _ _ _ _.
+  Let tyList : typ -> typ := @typ1 _ _ _ _.
   
   Lemma lf_nil_func_eq (t : typ) (f : func) (df : typD (tyList t))
     (Ho : listS f = Some (pNil t))
@@ -677,139 +373,6 @@ Section MakeListFuncSound.
    erewrite <- lf_cons_func_eq; try eassumption; reflexivity.
   Qed.
 
-  Lemma lf_length_func_eq (t : typ) (f : func) (df : typD (tyArr (tyList t) tyNat))
-    (Ho : listS f = Some (pLength t))
-    (Hf : funcAs f (tyArr (tyList t) tyNat) = Some df) :
-    df = lengthD t.
-  Proof.
-   rewrite (lf_funcAsOk _ Ho) in Hf.
-   unfold funcAs in Hf; simpl in *.
-   rewrite type_cast_refl in Hf; [|apply HROk].
-   unfold Rcast, Relim_refl in Hf.
-   inversion Hf. reflexivity.
-  Qed.
-
-  Lemma lf_length_eq tus tvs (t : typ) (e : expr typ func) (df : ExprI.exprT tus tvs (typD (tyArr (tyList t) tyNat)))
-    (Ho : listS e = Some (pLength t))
-    (Hf : exprD' tus tvs (tyArr (tyList t) tyNat) e = Some df) :
-    df = fun us vs => lengthD t.
-  Proof.
-   destruct e; simpl in *; try congruence.
-   autorewrite with exprD_rw in Hf; simpl in Hf; forward; inv_all; subst.
-   erewrite <- lf_length_func_eq; try eassumption; reflexivity.
-  Qed.
-
-  Lemma lf_NoDup_func_eq (t : typ) (f : func) (df : typD (tyArr (tyList t) tyProp))
-    (Ho : listS f = Some (pNoDup t))
-    (Hf : funcAs f (tyArr (tyList t) tyProp) = Some df) :
-    df = NoDupD t.
-  Proof.
-   rewrite (lf_funcAsOk _ Ho) in Hf.
-   unfold funcAs in Hf; simpl in *.
-   rewrite type_cast_refl in Hf; [|apply HROk].
-   unfold Rcast, Relim_refl in Hf.
-   inversion Hf. reflexivity.
-  Qed.
-
-  Lemma lf_NoDup_eq tus tvs (t : typ) (e : expr typ func) (df : ExprI.exprT tus tvs (typD (tyArr (tyList t) tyProp)))
-    (Ho : listS e = Some (pNoDup t))
-    (Hf : exprD' tus tvs (tyArr (tyList t) tyProp) e = Some df) :
-    df = fun us vs => NoDupD t.
-  Proof.
-   destruct e; simpl in *; try congruence.
-   autorewrite with exprD_rw in Hf; simpl in Hf; forward; inv_all; subst.
-   erewrite <- lf_NoDup_func_eq; try eassumption; reflexivity.
-  Qed.
-
-  Lemma lf_In_func_eq (t : typ) (f : func) (df : typD (tyArr t (tyArr (tyList t) tyProp)))
-    (Ho : listS f = Some (pIn t))
-    (Hf : funcAs f (tyArr t (tyArr (tyList t) tyProp)) = Some df) :
-    df = InD t.
-  Proof.
-   rewrite (lf_funcAsOk _ Ho) in Hf.
-   unfold funcAs in Hf; simpl in *.
-   rewrite type_cast_refl in Hf; [|apply HROk].
-   unfold Rcast, Relim_refl in Hf.
-   inversion Hf. reflexivity.
-  Qed.
-
-  Lemma lf_In_eq tus tvs (t : typ) (e : expr typ func) (df : ExprI.exprT tus tvs (typD (tyArr t (tyArr (tyList t) tyProp))))
-    (Ho : listS e = Some (pIn t))
-    (Hf : exprD' tus tvs (tyArr t (tyArr (tyList t) tyProp)) e = Some df) :
-    df = fun us vs => InD t.
-  Proof.
-   destruct e; simpl in *; try congruence.
-   autorewrite with exprD_rw in Hf; simpl in Hf; forward; inv_all; subst.
-   erewrite <- lf_In_func_eq; try eassumption; reflexivity.
-  Qed.
-
-  Lemma lf_map_func_eq (t u : typ) (f : func) (df : typD (tyArr (tyArr t u) (tyArr (tyList t) (tyList u))))
-    (Ho : listS f = Some (pMap t u))
-    (Hf : funcAs f (tyArr (tyArr t u) (tyArr (tyList t) (tyList u))) = Some df) :
-    df = mapD t u.
-  Proof.
-   rewrite (lf_funcAsOk _ Ho) in Hf.
-   unfold funcAs in Hf; simpl in *.
-   rewrite type_cast_refl in Hf; [|apply HROk].
-   unfold Rcast, Relim_refl in Hf.
-   inversion Hf. reflexivity.
-  Qed.
-
-  Lemma lf_map_eq tus tvs (t u : typ) (e : expr typ func) (df : ExprI.exprT tus tvs (typD (tyArr (tyArr t u) (tyArr (tyList t) (tyList u)))))
-    (Ho : listS e = Some (pMap t u))
-    (Hf : exprD' tus tvs (tyArr (tyArr t u) (tyArr (tyList t) (tyList u))) e = Some df) :
-    df = fun us vs => mapD t u.
-  Proof.
-   destruct e; simpl in *; try congruence.
-   autorewrite with exprD_rw in Hf; simpl in Hf; forward; inv_all; subst.
-   erewrite <- lf_map_func_eq; try eassumption; reflexivity.
-  Qed.
-
-  Lemma lf_fold_func_eq (t u : typ) (f : func) (df : typD (tyArr (tyArr u (tyArr t t)) (tyArr t (tyArr (tyList u) t))))
-    (Ho : listS f = Some (pFold t u))
-    (Hf : funcAs f (tyArr (tyArr u (tyArr t t)) (tyArr t (tyArr (tyList u) t))) = Some df) :
-    df = foldD t u.
-  Proof.
-   rewrite (lf_funcAsOk _ Ho) in Hf.
-   unfold funcAs in Hf; simpl in *.
-   rewrite type_cast_refl in Hf; [|apply HROk].
-   unfold Rcast, Relim_refl in Hf.
-   inversion Hf. reflexivity.
-  Qed.
-
-  Lemma lf_fold_eq (t u : typ) tus tvs (e : expr typ func) 
-    (df : ExprI.exprT tus tvs (typD (tyArr (tyArr u (tyArr t t)) (tyArr t (tyArr (tyList u) t)))))
-    (Ho : listS e = Some (pFold t u))
-    (Hf : exprD' tus tvs (tyArr (tyArr u (tyArr t t)) (tyArr t (tyArr (tyList u) t))) e = Some df) :
-    df = fun us vs => foldD t u.
-  Proof.
-   destruct e; simpl in *; try congruence.
-   autorewrite with exprD_rw in Hf; simpl in Hf; forward; inv_all; subst.
-   erewrite <- lf_fold_func_eq; try eassumption; reflexivity.
-  Qed.
-
-  Lemma lf_zip_func_eq (t u : typ) (f : func) (df : typD (tyArr (tyList t) (tyArr (tyList u) (tyList (tyProd t u)))))
-    (Ho : listS f = Some (pZip t u))
-    (Hf : funcAs f (tyArr (tyList t) (tyArr (tyList u) (tyList (tyProd t u)))) = Some df) :
-    df = zipD t u.
-  Proof.
-   rewrite (lf_funcAsOk _ Ho) in Hf.
-   unfold funcAs in Hf; simpl in *.
-   rewrite type_cast_refl in Hf; [|apply HROk].
-   unfold Rcast, Relim_refl in Hf.
-   inversion Hf. reflexivity.
-  Qed.
-
-  Lemma lf_zip_eq tus tvs (t u : typ) (e : expr typ func) (df : ExprI.exprT tus tvs (typD (tyArr (tyList t) (tyArr (tyList u) (tyList (tyProd t u))))))
-    (Ho : listS e = Some (pZip t u))
-    (Hf : exprD' tus tvs (tyArr (tyList t) (tyArr (tyList u) (tyList (tyProd t u)))) e = Some df) :
-    df = fun us vs => zipD t u.
-  Proof.
-   destruct e; simpl in *; try congruence.
-   autorewrite with exprD_rw in Hf; simpl in Hf; forward; inv_all; subst.
-   erewrite <- lf_zip_func_eq; try eassumption; reflexivity.
-  Qed.
-
   Lemma mkNil_sound (t : typ) tus tvs :
     exprD' tus tvs (tyList t) (mkNil t) = Some (fun _ _ => nilD t).
   Proof.
@@ -838,185 +401,30 @@ Section MakeListFuncSound.
     rewrite type_cast_refl; [reflexivity | apply _].
   Qed.
 
-  Lemma mkConsD (t : typ) (tus tvs : tenv typ) x xs (lstD : ExprI.exprT tus tvs (typD (tyList t)))
-    (H : exprD' tus tvs (tyList t) (mkCons t x xs) = Some lstD) : 
-    match exprD' tus tvs t x with
-      | Some xD => 
-        match exprD' tus tvs (tyList t) xs with
-          | Some xsD => lstD = exprT_App (exprT_App (fun _ _ => consD t) xD) xsD
-          | None => False
-        end
-      | None => False
-    end.
-  Proof.
-    unfold mkCons in H.
-    autorewrite with exprD_rw in H; simpl in H; forward; inv_all; subst.
-    autorewrite with exprD_rw in H0; simpl in H0; forward; inv_all; subst.
-    autorewrite with exprD_rw in H2; simpl in H2; forward; inv_all; subst.
-    pose proof (lf_cons_func_type_eq _ _ (lf_fConsOk t) H2).
-    r_inj H4.
-    forward; inv_all; subst. 
-    pose proof (lf_cons_func_eq _ (lf_fConsOk t) H2); subst.
-    reflexivity.
-  Qed.
-
-  Lemma mkZipD (t u : typ) (tus tvs : tenv typ) xs ys (lstD : ExprI.exprT tus tvs (typD (tyList (tyProd t u))))
-    (H : exprD' tus tvs (tyList (tyProd t u)) (mkZip t u xs ys) = Some lstD) : 
-    match exprD' tus tvs (tyList t) xs with
-      | Some xsD => 
-        match exprD' tus tvs (tyList u) ys with
-          | Some ysD => lstD = exprT_App (exprT_App (fun _ _ => zipD t u) xsD) ysD
-          | None => False
-        end
-      | None => False
-    end.
-  Proof.
-    unfold mkZip in H.
-    autorewrite with exprD_rw in H; simpl in H; forward; inv_all; subst.
-    autorewrite with exprD_rw in H0; simpl in H0; forward; inv_all; subst.
-    autorewrite with exprD_rw in H2; simpl in H2; forward; inv_all; subst.
-    pose proof (lf_zip_func_type_eq _ _ (lf_fZipOk t u) H2).
-    r_inj H4.
-    forward; inv_all; subst. 
-    pose proof (lf_zip_func_eq _ (lf_fZipOk t u) H2); subst.
-    reflexivity.
-  Qed.
-
-  Lemma mkLength_sound (t : typ) (tus tvs : tenv typ) lst
-    (lstD : ExprI.exprT tus tvs (typD (tyList t))) 
-    (Hlst : exprD' tus tvs (tyList t) lst = Some lstD)  :
-    exprD' tus tvs tyNat (mkLength t lst) = Some (exprT_App (fun _ _ => lengthD t) lstD).
-  Proof.
-    unfold mkLength; simpl.
-    autorewrite with exprD_rw; simpl; forward; inv_all; subst.
-    rewrite (ExprTac.exprD_typeof_Some _ _ _ lst _ Hlst).
-    autorewrite with exprD_rw; simpl; forward; inv_all; subst.
-    pose proof (lf_fLengthOk t) as Ho.
-    pose proof (lf_funcAsOk _ Ho) as H1.
-    rewrite H1. unfold funcAs; simpl.
-    rewrite type_cast_refl; [reflexivity | apply _].
-  Qed.
-
-  Lemma mkNoDup_sound (t : typ) (tus tvs : tenv typ) lst
-    (lstD : ExprI.exprT tus tvs (typD (tyList t))) 
-    (Hlst : exprD' tus tvs (tyList t) lst = Some lstD)  :
-    exprD' tus tvs tyProp (mkNoDup t lst) = Some (exprT_App (fun _ _ => NoDupD t) lstD).
-  Proof.
-    unfold mkNoDup; simpl.
-    autorewrite with exprD_rw; simpl; forward; inv_all; subst.
-    rewrite (ExprTac.exprD_typeof_Some _ _ _ lst _ Hlst).
-    autorewrite with exprD_rw; simpl; forward; inv_all; subst.
-    pose proof (lf_fNoDupOk t) as Ho.
-    pose proof (lf_funcAsOk _ Ho) as H1.
-    rewrite H1. unfold funcAs; simpl.
-    rewrite type_cast_refl; [reflexivity | apply _].
-  Qed.
-
-  Lemma mkIn_sound (t : typ) (tus tvs : tenv typ) x lst
-    (xD : ExprI.exprT tus tvs (typD t)) 
-    (lstD : ExprI.exprT tus tvs (typD (tyList t))) 
-    (Hx : exprD' tus tvs t x = Some xD) 
-    (Hlst : exprD' tus tvs (tyList t) lst = Some lstD)  :
-    exprD' tus tvs tyProp (mkIn t x lst) = Some (exprT_App (exprT_App (fun _ _ => InD t) xD) lstD).
-  Proof.
-    unfold mkIn; simpl.
-    autorewrite with exprD_rw; simpl; forward; inv_all; subst.
-    rewrite (ExprTac.exprD_typeof_Some _ _ _ lst _ Hlst).
-    autorewrite with exprD_rw; simpl; forward; inv_all; subst.
-    rewrite (ExprTac.exprD_typeof_Some _ _ _ x _ Hx).
-    autorewrite with exprD_rw; simpl; forward; inv_all; subst.
-    pose proof (lf_fInOk t) as Ho.
-    pose proof (lf_funcAsOk _ Ho) as H1.
-    rewrite H1. unfold funcAs; simpl.
-    rewrite type_cast_refl; [reflexivity | apply _].
-  Qed.
-
-  Lemma mkMap_sound (t u : typ) (tus tvs : tenv typ) f lst
-    (fD : ExprI.exprT tus tvs (typD (tyArr t u)))
-    (lstD : ExprI.exprT tus tvs (typD (tyList t))) 
-    (Hf : exprD' tus tvs (tyArr t u) f = Some fD) 
-    (Hlst : exprD' tus tvs (tyList t) lst = Some lstD)  :
-    exprD' tus tvs (tyList u) (mkMap t u f lst) = Some (exprT_App (exprT_App (fun _ _ => mapD t u) fD) lstD).
-  Proof.
-    unfold mkMap; simpl.
-    autorewrite with exprD_rw; simpl; forward; inv_all; subst.
-    rewrite (ExprTac.exprD_typeof_Some _ _ _ lst _ Hlst).
-    autorewrite with exprD_rw; simpl; forward; inv_all; subst.
-    rewrite (ExprTac.exprD_typeof_Some _ _ _ f _ Hf).
-    autorewrite with exprD_rw; simpl; forward; inv_all; subst.
-    pose proof (lf_fMapOk t u) as Ho.
-    pose proof (lf_funcAsOk _ Ho) as H1.
-    rewrite H1. unfold funcAs; simpl.
-    rewrite type_cast_refl; [reflexivity | apply _].
-  Qed.
-
-  Lemma mkFold_sound (t u : typ) (tus tvs : tenv typ) f acc lst
-    (fD : ExprI.exprT tus tvs (typD (tyArr u (tyArr t t))))
-    (accD : ExprI.exprT tus tvs (typD t))
-    (lstD : ExprI.exprT tus tvs (typD (tyList u))) 
-    (Hf : exprD' tus tvs (tyArr u (tyArr t t)) f = Some fD) 
-    (Hacc : exprD' tus tvs t acc = Some accD)
-    (Hlst : exprD' tus tvs (tyList u) lst = Some lstD)  :
-    exprD' tus tvs t (mkFold t u f acc lst) = Some (exprT_App (exprT_App (exprT_App (fun _ _ => foldD t u) fD) accD) lstD).
-  Proof.
-    unfold mkFold; simpl.
-    autorewrite with exprD_rw; simpl; forward; inv_all; subst.
-    rewrite (ExprTac.exprD_typeof_Some _ _ _ lst _ Hlst).
-    autorewrite with exprD_rw; simpl; forward; inv_all; subst.
-    rewrite (ExprTac.exprD_typeof_Some _ _ _ acc _ Hacc).
-    autorewrite with exprD_rw; simpl; forward; inv_all; subst.
-    rewrite (ExprTac.exprD_typeof_Some _ _ _ f _ Hf).
-    autorewrite with exprD_rw; simpl; forward; inv_all; subst.
-    pose proof (lf_fFoldOk t u) as Ho.
-    pose proof (lf_funcAsOk _ Ho) as H2.
-    rewrite H2. unfold funcAs; simpl.
-    rewrite type_cast_refl; [reflexivity | apply _].
-  Qed.
-
-  Lemma mkZip_sound (t u : typ) (tus tvs : tenv typ) xs ys
-    (xsD : ExprI.exprT tus tvs (typD (tyList t))) 
-    (ysD : ExprI.exprT tus tvs (typD (tyList u))) 
-    (Hxs : exprD' tus tvs (tyList t) xs = Some xsD) 
-    (Hys : exprD' tus tvs (tyList u) ys = Some ysD) :
-    exprD' tus tvs (tyList (tyProd t u)) (mkZip t u xs ys) = 
-      Some (exprT_App (exprT_App (fun _ _ => zipD t u) xsD) ysD).
-  Proof.
-    unfold mkZip; simpl.
-    autorewrite with exprD_rw; simpl; forward; inv_all; subst.
-    rewrite (ExprTac.exprD_typeof_Some _ _ _ ys _ Hys).
-    autorewrite with exprD_rw; simpl; forward; inv_all; subst.
-    rewrite (ExprTac.exprD_typeof_Some _ _ _ xs _ Hxs).
-    autorewrite with exprD_rw; simpl; forward; inv_all; subst.
-    pose proof (lf_fZipOk t u) as Ho.
-    pose proof (lf_funcAsOk _ Ho) as H1.
-    rewrite H1. unfold funcAs; simpl.
-    rewrite type_cast_refl; [reflexivity | apply _].
-  Qed.
-
 End MakeListFuncSound.
 
 Section ListCases.
   Context {typ func : Type} {LF : ListFunc typ func}.
 
-  Definition list_cases (e : expr typ func) (P : expr typ func -> Type)
-    (f_nil : forall t f, listS f = Some (pNil t) -> P (Inj f)) 
-    (f_cons : forall t f x xs, listS f = Some (pCons t) -> P (App (App (Inj f) x) xs))
-    (f_default : P e) : P e := 
-    match e as e' return e = e' -> P e with
+  Definition list_cases (e : expr typ func) (P : Type)
+    (f_nil : P)
+    (f_cons : expr typ func -> expr typ func -> P)
+    (f_default : P) : P := 
+    match e as e' return e = e' -> P with
       | Inj f => 
-        match listS f as e'' return listS f = e'' -> e = Inj f -> P e with
+        match listS f as e'' return listS f = e'' -> e = Inj f -> P with
           | Some p => 
-            match p as p' return listS f = Some p' -> e = Inj f -> P e with
-              | pNil t => fun eq1 eq2 => eq_rect_r P (f_nil t f eq1) eq2
+            match p as p' return listS (ListFunc := LF) (typ := typ) f = Some p' -> e = Inj f -> P with
+              | pNil t => fun _ _ => f_nil
               | _ => fun _ _ => f_default
             end
           | _ => fun _ _ => f_default
         end eq_refl
       | App (App (Inj f) x) xs =>
-        match listS f as e'' return listS f = e'' -> e = App (App (Inj f) x) xs -> P e with
+        match listS f as e'' return listS f = e'' -> e = App (App (Inj f) x) xs -> P with
           | Some p => 
-            match p as p' return listS f = Some p' -> e = App (App (Inj f) x) xs -> P e with
-              | pCons t => fun eq1 eq2 => eq_rect_r P (f_cons t f x xs eq1) eq2
+            match p as p' return listS (ListFunc := LF) (typ := typ) f = Some p' -> e = App (App (Inj f) x) xs -> P with
+              | pCons t => fun _ _ => f_cons x xs
               | _ => fun _ _ => f_default
             end
           | _ => fun _ _ => f_default
@@ -1026,159 +434,72 @@ Section ListCases.
     
   Fixpoint list_length (e : expr typ func) : nat :=
     @list_cases e _
-      (fun _ _ _ => 0)
-      (fun _ _ _ xs _ => S (list_length xs))
+      0
+      (fun _ xs => S (list_length xs))
       0.
     
 End ListCases.      
 
 Section ListCasesRules.
-  Context {typ func : Type} {LF : ListFunc typ func} {LT : ListType typ}.
-  Context {BF : BaseFunc typ func} {BT : BaseType typ}.
+  Context {typ func : Type} {LF : ListFunc typ func}.
   Context {RType_typ : RType typ} {RTypeOk_typ : RTypeOk} {RSym_func : RSym func}.
-  Context {LTD : ListTypeD LT} {BTD : BaseTypeD BT}.
   
   Context {HEq : RelDec (@eq typ)}.
     
   Context {Typ2_tyArr : Typ2 _ Fun}.
-  Context {Typ0_tyProp : Typ0 _ Prop}.
+  Context {Typ1_tyList : Typ1 _ list}.
  
   Context {LFOk : ListFuncOk typ func}.
 
-  Lemma list_case tus tvs (t : typ) (e : expr typ func) (P : expr typ func -> Type) (Q : forall e, P e -> Prop)
-    (f_nil : forall t f, listS f = Some (pNil t) -> P (Inj f)) 
-    (f_cons : forall t f x xs, listS f = Some (pCons t) -> P (App (App (Inj f) x) xs))
-    (f_default : P e) 
+  Context {Typ2Ok_tyArr : Typ2Ok Typ2_tyArr}.
+  Context {Typ1Ok_tyList : Typ1Ok Typ1_tyList}.
+  Context {RSym_funcOk : RSymOk RSym_func}.
+
+  Let tyList : typ -> typ  := @typ1 _ _ _ _.
+
+  Lemma list_case tus tvs (t : typ) (e : expr typ func) (P : Type) (Q : P -> Prop)
+    (f_nil : P) 
+    (f_cons : expr typ func -> expr typ func -> P)
+    (f_default : P) 
     (HType : typeof_expr tus tvs e = Some (tyList t))
-    (Hdefault : Q e (f_default))
-    (Hnil : forall f (eq1 : listS f = Some (pNil t)), Q (Inj f) (f_nil t f eq1))
-    (Hcons : forall f x xs (eq1 : listS f = Some (pCons t)), Q (App (App (Inj f) x) xs) (f_cons t f x xs eq1)) : 
-    	(Q e (@list_cases typ func LF e P f_nil f_cons f_default)).
+    (Hdefault : Q f_default)
+    (Hnil : forall f, listS f = Some (pNil t) -> e = Inj f -> Q f_nil)
+    (Hcons : forall f x xs, 
+               listS f = Some (pCons t) -> e = App (App (Inj f) x) xs ->
+               typeof_expr tus tvs x = Some t -> typeof_expr tus tvs xs = Some (tyList t) ->
+               TransitiveClosure.leftTrans (expr_acc (func := func)) x e ->
+               TransitiveClosure.leftTrans (expr_acc (func := func)) xs e ->
+               Q (f_cons x xs)) : 
+    (Q (@list_cases typ func LF e P f_nil f_cons f_default)).
   Proof.
     destruct e; simpl; try apply Hdefault.
     { 
-      generalize (@eq_refl _ (listS f)).
-      
-      change (let x := listS f in 
-              forall e : listS f = x,
-                Q (Inj f)
-                  (match
-                      x as e'' return (listS f = e'' -> Inj f = Inj f -> P (Inj f))
-                    with
-                      | Some p =>
-                        match
-                          p as p' return (listS f = Some p' -> Inj f = Inj f -> P (Inj f))
-                        with
-                          | pNil t0 =>
-                            fun (eq1 : listS f = Some (pNil t0)) (eq2 : Inj f = Inj f) =>
-                              eq_rect_r P (f_nil t0 f eq1) eq2
-                          | pCons y =>
-                            fun (_ : listS f = Some (pCons y)) (_ : Inj f = Inj f) =>
-                              f_default
-                          | pLength y =>
-                            fun (_ : listS f = Some (pLength y)) (_ : Inj f = Inj f) =>
-                              f_default
-                          | pNoDup y =>
-                            fun (_ : listS f = Some (pNoDup y)) (_ : Inj f = Inj f) =>
-                              f_default
-                          | pIn y =>
-                            fun (_ : listS f = Some (pIn y)) (_ : Inj f = Inj f) =>
-                              f_default
-                          | pMap y y0 =>
-                            fun (_ : listS f = Some (pMap y y0)) (_ : Inj f = Inj f) =>
-                              f_default
-                          | pFold y y0 =>
-                            fun (_ : listS f = Some (pFold y y0)) (_ : Inj f = Inj f) =>
-                              f_default
-                          | pZip y y0 =>
-                            fun (_ : listS f = Some (pZip y y0)) (_ : Inj f = Inj f) =>
-                              f_default
-                        end
-                      | None => fun (_ : listS f = None) (_ : Inj f = Inj f) => f_default
-                    end e eq_refl)).
-      destruct x; intros; try apply Hdefault.
-      destruct l eqn:Heq; intros; try apply Hdefault.
+      destruct (listS f) eqn:Heq1; try apply Hdefault.
+      destruct l eqn:Heq2; try apply Hdefault.
       simpl in HType.
-      pose proof (lf_funcAsOk f e).
-      specialize (H (tyList t0)).
-      simpl in H.
-      unfold funcAs at 2 in H.
-      simpl in H.
-      rewrite type_cast_refl in H.
-      simpl in H.
-      unfold Rrefl, Rcast, Relim, Rsym in H.
-      simpl in H.
-      pose proof (typeof_funcAs f (tyList t0) H).
-      rewrite H0 in HType.
-      inversion HType; subst. apply tyList_inj in H2; unfold Rty in H2. subst.
-      apply Hnil. apply _.
-   } {
-     destruct e1; try apply Hdefault.
-     destruct e1_1; try apply Hdefault.
-     generalize (@eq_refl _ (listS f)).
-	 change (let x := listS f in
-	 forall e : listS f = x,
-Q
-  (
-  match
-     x as e''
-     return
-       (listS f = e'' ->
-        App (App (Inj f) e1_2) e2 = App (App (Inj f) e1_2) e2 ->
-        P (App (App (Inj f) e1_2) e2))
-   with
-   | Some p =>
-       match
-         p as p'
-         return
-           (listS f = Some p' ->
-            App (App (Inj f) e1_2) e2 = App (App (Inj f) e1_2) e2 ->
-            P (App (App (Inj f) e1_2) e2))
-       with
-       | pNil y =>
-           fun (_ : listS f = Some (pNil y))
-             (_ : App (App (Inj f) e1_2) e2 = App (App (Inj f) e1_2) e2) =>
-           f_default
-       | pCons t0 =>
-           fun (eq1 : listS f = Some (pCons t0))
-             (eq2 : App (App (Inj f) e1_2) e2 = App (App (Inj f) e1_2) e2) =>
-           f_cons t0 f e1_2 e2 eq1 eq2
-       | pLength y =>
-           fun (_ : listS f = Some (pLength y))
-             (_ : App (App (Inj f) e1_2) e2 = App (App (Inj f) e1_2) e2) =>
-           f_default
-       | pNoDup y =>
-           fun (_ : listS f = Some (pNoDup y))
-             (_ : App (App (Inj f) e1_2) e2 = App (App (Inj f) e1_2) e2) =>
-           f_default
-       | pIn y =>
-           fun (_ : listS f = Some (pIn y))
-             (_ : App (App (Inj f) e1_2) e2 = App (App (Inj f) e1_2) e2) =>
-           f_default
-       | pMap y y0 =>
-           fun (_ : listS f = Some (pMap y y0))
-             (_ : App (App (Inj f) e1_2) e2 = App (App (Inj f) e1_2) e2) =>
-           f_default
-       | pFold y y0 =>
-           fun (_ : listS f = Some (pFold y y0))
-             (_ : App (App (Inj f) e1_2) e2 = App (App (Inj f) e1_2) e2) =>
-           f_default
-       | pZip y y0 =>
-           fun (_ : listS f = Some (pZip y y0))
-             (_ : App (App (Inj f) e1_2) e2 = App (App (Inj f) e1_2) e2) =>
-           f_default
-       end
-   | None =>
-       fun (_ : listS f = None)
-         (_ : App (App (Inj f) e1_2) e2 = App (App (Inj f) e1_2) e2) =>
-       f_default
-   end e eq_refl)
-	 ).
-	 destruct x; intros; try apply Hdefault.
-	 destruct l eqn:Heq; try apply Hdefault.
-	 simpl in HType.
-	 admit.	 
-   }
- Admitted.
+      pose proof (list_nil_type_eq f Heq1 HType).
+      apply typ1_inj in H; [|apply _]; unfold Rty in H; subst.
+      eapply Hnil; [eassumption | reflexivity].
+    } {
+      destruct e1; simpl; try apply Hdefault.
+      destruct e1_1; simpl; try apply Hdefault.
+      destruct (listS f) eqn:Heq1; try apply Hdefault.
+      destruct l eqn:Heq2; try apply Hdefault. subst.
+      simpl in HType.
+      forward.
+      pose proof (list_cons_type_eq f Heq1 H); subst.
+      
+      apply ExprFacts.type_of_apply_Some in H2.
+      apply typ2_inj in H2; [|apply _]; unfold Rty in H2; destruct H2; subst.
+      apply ExprFacts.type_of_apply_Some in HType.
+      apply typ2_inj in HType; [|apply _]; unfold Rty in HType; destruct HType; subst.
+      apply typ1_inj in H3; [|apply _]; unfold Rty in H3; subst.
+      
+      eapply Hcons; try eassumption. 
+      { reflexivity. }
+      { apply TransitiveClosure.LTStep with (App (Inj f) e1_2); repeat constructor. }
+      { repeat constructor. }
+    }
+  Qed.
  
 End ListCasesRules.
