Charge!/src/Charge/ModularFunc/ProdFunc.v
@@ -36,32 +36,34 @@ Class PairFunc (typ func : Type) := {
 }.
 
 Section PairFuncSum.
-	Context {typ func : Type} {H : PairFunc typ func}.
+  Context {typ func : Type} {H : PairFunc typ func}.
 	
-	Global Instance PairFuncPMap (p : positive) (m : pmap Type) 
-	  (pf : Some func = pmap_lookup' m p) :
-	  PairFunc typ (OneOf m) := {
-	    fPair t u := Into (fPair t u) p pf;
-	    
-	    pairS f :=
-	      match f with
-	        | Build_OneOf _ p' pf1 =>
-	          match Pos.eq_dec p p' with
-	            | left Heq => 
-	              pairS (eq_rect_r (fun o => match o with | Some T => T | None => Empty_set end) pf1 
-	                (eq_rect _ (fun p =>  Some func = pmap_lookup' m p) pf _ Heq))
-	            | right _ => None
-	          end
-	      end
-	}.
+  Global Instance PairFuncPMap (p : positive) (m : pmap Type) 
+	 (pf : Some func = pmap_lookup' m p) :
+    PairFunc typ (OneOf m) := 
+    {
+      fPair t u := Into (fPair t u) p pf;
+      
+      pairS f :=
+	match f with
+	  | Build_OneOf _ p' pf1 =>
+	    match Pos.eq_dec p p' with
+	      | left Heq => 
+	        pairS (eq_rect_r (fun o => match o with | Some T => T | None => Empty_set end) pf1 
+	                         (eq_rect _ (fun p =>  Some func = pmap_lookup' m p) pf _ Heq))
+	      | right _ => None
+	    end
+	end
+    }.
 
-    Global Instance PairFuncExpr :
-    	PairFunc typ (expr typ func) := {
-    	  fPair t1 t2 := Inj (fPair t1 t2);
-    	  pairS f := match f with
-    	  	       | Inj f => pairS f
-    	  	       | _     => None
-    	  	     end
+  Global Instance PairFuncExpr :
+    PairFunc typ (expr typ func) := 
+    {
+      fPair t1 t2 := Inj (fPair t1 t2);
+      pairS f := match f with
+    	  	   | Inj f => pairS f
+    	  	   | _     => None
+    	  	 end
     }.
 
 End PairFuncSum.
@@ -71,17 +73,18 @@ Section PairFuncInst.
   Context {func : Type} {H : PairFunc typ func}.
   Context {RelDec_typ : RelDec (@eq typ)}.
   Context {RelDecCorrect_typ : RelDec_Correct RelDec_typ}.
-
+  
   Context {Typ2_tyArr : Typ2 _ Fun}.
   Context {Typ2_tyProd : Typ2 _ prod}.
-
+  
   Let tyArr : typ -> typ -> typ := @typ2 _ _ _ Typ2_tyArr.
   Let tyProd : typ -> typ -> typ := @typ2 _ _ _ Typ2_tyProd.
 
-  Global Instance PairFuncInst : PairFunc typ (pair_func typ) := {
-	fPair := pPair;
-	pairS f := Some f 
-  }.
+  Global Instance PairFuncInst : PairFunc typ (pair_func typ) := 
+    {
+      fPair := pPair;
+      pairS f := Some f 
+    }.
 
   Definition typeof_pair_func pf :=
     match pf with
@@ -98,16 +101,17 @@ Section PairFuncInst.
     typD (tyProd t u) = (A * B)%type :=
     eq_ind (typD t) (fun X : Type => typD (tyProd t u) = (X * B)%type)
       (eq_ind (typD u) (fun Y : Type => typD (tyProd t u) = (typD t * Y)%type)
-         (typ2_cast t u) B e2) A e1.
-    
-
+              (typ2_cast t u) B e2) A e1.
+  
+  
   Definition prodD t u (p : typD (tyProd t u)) : typD t * typD u :=
     trmD p (pairE (t := t) (u := u) eq_refl eq_refl).
-	  
+  
   Definition prodR t u (p : typD t * typD u) : typD (tyProd t u) :=
     trmR p (pairE (t := t) (u := u) eq_refl eq_refl).
-
-  Lemma prodDR (t u : typ) A B C D (x : A) (y : B) (e1 : typD t = A) (e2 : typD u = B) (e3 : typD t = C) (e4 : typD u = D) :
+  
+  Lemma prodDR (t u : typ) A B C D (x : A) (y : B) (e1 : typD t = A) 
+        (e2 : typD u = B) (e3 : typD t = C) (e4 : typD u = D) :
     trmD (trmR (x, y) (pairE e1 e2)) (pairE e3 e4) = 
     (trmD (trmR x e1) e3, trmD (trmR y e2) e4).
   Proof.
@@ -126,7 +130,7 @@ Section PairFuncInst.
 
   Definition pairD (t u : typ) : typD (tyArr t (tyArr u (tyProd t u))) :=
     (tyArrR2 (fun a b => prodR t u (a, b))).
-
+  
   Definition pair_func_symD bf :=
     match bf as bf return match typeof_pair_func bf return Type with
 			    | Some t => typD t
@@ -142,7 +146,7 @@ Section PairFuncInst.
       symD := pair_func_symD ;
       sym_eqb := pair_func_eq
     }.
-
+  
   Global Instance RSymOk_PairFunc : SymI.RSymOk RSym_PairFunc.
   Proof.
     split; intros.
@@ -150,15 +154,15 @@ Section PairFuncInst.
     + consider (t ?[ eq ] t1 && t0 ?[ eq ] t2)%bool;
       intuition congruence.
   Qed.
-
+  
 End PairFuncInst.
 
 Section MakePair.
-	Context {typ func : Type} {RType_typ : RType typ}.
-	Context {HF : PairFunc typ func}.
-
-	Definition mkPair t u a b := App (App (fPair t u) a) b.
-
+  Context {typ func : Type} {RType_typ : RType typ}.
+  Context {HF : PairFunc typ func}.
+  
+  Definition mkPair t u a b := App (App (fPair t u) a) b.
+  
 End MakePair.
 
 Section PairFuncOk.
@@ -166,37 +170,39 @@ Section PairFuncOk.
   Context {BF: PairFunc typ func} {RSym_func : RSym func}.
   Context {RelDec_eq : RelDec (@eq typ)}.
   Context {RelDec_eqOk : RelDec_Correct RelDec_eq}.
-
+  
   Context {Typ2_tyArr : Typ2 _ Fun}.
   Context {Typ2_tyProd : Typ2 _ prod}.
-
-  Class PairFuncOk := {
-    bf_funcAsOk (f : func) (e : @pair_func typ) : 
-      pairS f = Some e -> 
-      forall t, funcAs f t = 
-                funcAs (RSym_func := RSym_PairFunc) e t;
-    bf_fPairOk t u : pairS (fPair t u) = Some (pPair t u)
-  }.
-
+  
+  Class PairFuncOk := 
+    {
+      bf_funcAsOk (f : func) (e : @pair_func typ) : 
+        pairS f = Some e -> 
+        forall t, funcAs f t = 
+                  funcAs (RSym_func := RSym_PairFunc) e t;
+      bf_fPairOk t u : pairS (fPair t u) = Some (pPair t u)
+    }.
+  
 End PairFuncOk.
 
 Implicit Arguments PairFuncOk [[BF] [RType_typ] [RSym_func] [RelDec_eq]
-                               [Typ2_tyArr] [Typ2_tyProd]].
+                                    [Typ2_tyArr] [Typ2_tyProd]].
 
 Section PairFuncBaseOk.
   Context {typ func : Type} {RType_typ : RType typ}.
   Context {BF: PairFunc typ func} {RSym_func : RSym func}.
   Context {RelDec_eq : RelDec (@eq typ)}.
   Context {RelDec_eqOk : RelDec_Correct RelDec_eq}.
-
+  
   Context {Typ2_tyArr : Typ2 _ Fun}.
   Context {Typ2_Pair : Typ2 _ prod}.
-
+  
   Global Program Instance PairFuncBaseOk : 
-  	PairFuncOk typ (RSym_func := RSym_PairFunc) (pair_func typ) := {
-    bf_funcAsOk := fun _ _ _ _ => eq_refl;
-    bf_fPairOk t u := eq_refl
-  }.
+    PairFuncOk typ (RSym_func := RSym_PairFunc) (pair_func typ) := 
+    {
+      bf_funcAsOk := fun _ _ _ _ => eq_refl;
+      bf_fPairOk t u := eq_refl
+    }.
 
 End PairFuncBaseOk.
 
@@ -204,13 +210,13 @@ Section PairFuncExprOk.
   Context {typ func : Type} `{HOK : PairFuncOk typ func}.
   Context {HROk : RTypeOk}.
   Context {A : Type} {RSymA : RSym A}.
-
+  
   Context {Typ2_tyArrOk : Typ2Ok Typ2_tyArr}
           {RSym_funcOk : RSymOk RSym_func0}.
-
+  
   Let tyArr : typ -> typ -> typ := @typ2 _ _ _ Typ2_tyArr.
   Let tyProd : typ -> typ -> typ := @typ2 _ _ _ Typ2_tyProd.
-
+  
   Lemma BaseFunc_typeOk (f : func) (e : pair_func typ) (H : pairS f = Some e) :
     typeof_sym f = typeof_pair_func e.
   Proof.
@@ -219,14 +225,14 @@ Section PairFuncExprOk.
     destruct e; simpl in *;
     match goal with 
       | |- typeof_sym ?f = Some ?t => 
-	 	specialize (H1 t);
-	 	simpl in H1;
-	 	unfold funcAs in H1; simpl in H1 ; rewrite type_cast_refl in H1; [|apply _];
-	    generalize dependent (symD f);
-	 	destruct (typeof_sym f); simpl; intros; [forward|]; inversion H1
- 	end.
+	specialize (H1 t);
+	  simpl in H1;
+	  unfold funcAs in H1; simpl in H1 ; rewrite type_cast_refl in H1; [|apply _];
+	  generalize dependent (symD f);
+	  destruct (typeof_sym f); simpl; intros; [forward|]; inversion H1
+    end.
   Qed.
-
+  
   Lemma bf_pair_func_type_eq (f : func) t u v df
         (H1 : pairS f = Some (pPair t u)) (H2 : funcAs f v = Some df) :
     v = tyArr t (tyArr u (tyProd t u)).
@@ -236,7 +242,7 @@ Section PairFuncExprOk.
     forward.
     rewrite <- r; reflexivity.
   Qed.
-
+  
   Lemma pair_func_type_eq (f : func) (t u v : typ) 
         (H1 : pairS f = Some (pPair t u)) (H2 : typeof_sym f = Some v) :
     v = tyArr t (tyArr u (tyProd t u)).
@@ -247,55 +253,56 @@ Section PairFuncExprOk.
     simpl in H. forward.
     eapply bf_pair_func_type_eq; eassumption.
   Qed.
-
+  
   Lemma bf_pair_type_eq tus tvs (e : expr typ func) t u v df
-    (H1 : pairS e = Some (pPair t u)) (H2 : exprD' tus tvs v e = Some df) :
+        (H1 : pairS e = Some (pPair t u)) (H2 : exprD' tus tvs v e = Some df) :
     v = tyArr t (tyArr u (tyProd t u)).
   Proof.
-   destruct e; simpl in *; try congruence.
-   autorewrite with exprD_rw in H2; simpl in H2; forward; inv_all; subst.
-   apply (bf_pair_func_type_eq _ _ H1 H).
+    destruct e; simpl in *; try congruence.
+    autorewrite with exprD_rw in H2; simpl in H2; forward; inv_all; subst.
+    apply (bf_pair_func_type_eq _ _ H1 H).
   Qed.
-
+  
 End PairFuncExprOk.
 
 Section MakePairFuncSound.
   Context {typ func : Type} `{HOK : PairFuncOk typ func}.
   Context {HROk : RTypeOk} {Typ2_tyArrOk : Typ2Ok Typ2_tyArr}
           {RSym_funcOk : RSymOk RSym_func0}.
-
+  
   Let tyArr : typ -> typ -> typ := @typ2 _ _ _ Typ2_tyArr.
   Let tyProd : typ -> typ -> typ := @typ2 _ _ _ Typ2_tyProd.
-
+  
   Lemma bf_pair_func_eq (t u : typ) (f : func) (fD : typD (tyArr t (tyArr u (tyProd t u))))
-    (Ho : pairS f = Some (pPair t u))
-    (Hf : funcAs f (tyArr t (tyArr u (tyProd t u))) = Some fD) :
+        (Ho : pairS f = Some (pPair t u))
+        (Hf : funcAs f (tyArr t (tyArr u (tyProd t u))) = Some fD) :
     fD = pairD t u.
   Proof.
-   rewrite (bf_funcAsOk _ Ho) in Hf.
-   unfold funcAs in Hf; simpl in *.
-   rewrite type_cast_refl in Hf; [|apply HROk].
-   unfold Rcast, Relim_refl in Hf.
-   inversion Hf. reflexivity.
+    rewrite (bf_funcAsOk _ Ho) in Hf.
+    unfold funcAs in Hf; simpl in *.
+    rewrite type_cast_refl in Hf; [|apply HROk].
+    unfold Rcast, Relim_refl in Hf.
+    inversion Hf. reflexivity.
   Qed.
-
+  
   Lemma bf_pair_eq tus tvs (t u : typ) (e : expr typ func) 
-    (eD : ExprI.exprT tus tvs (typD (tyArr t (tyArr u (tyProd t u)))))
-    (Ho : pairS e = Some (pPair t u))
-    (Hf : exprD' tus tvs (tyArr t (tyArr u (tyProd t u))) e = Some eD) :
+        (eD : ExprI.exprT tus tvs (typD (tyArr t (tyArr u (tyProd t u)))))
+        (Ho : pairS e = Some (pPair t u))
+        (Hf : exprD' tus tvs (tyArr t (tyArr u (tyProd t u))) e = Some eD) :
     eD = (fun us vs => pairD t u).
   Proof.
-   destruct e; simpl in *; try congruence.
-   autorewrite with exprD_rw in Hf; simpl in Hf; forward; inv_all; subst.
-   rewrite (bf_pair_func_eq _ Ho H); reflexivity.
+    destruct e; simpl in *; try congruence.
+    autorewrite with exprD_rw in Hf; simpl in Hf; forward; inv_all; subst.
+    rewrite (bf_pair_func_eq _ Ho H); reflexivity.
   Qed.
-
+  
   Lemma mkPair_sound (t u : typ) (tus tvs : tenv typ) a b
-    (aD : ExprI.exprT tus tvs (typD t)) 
-    (bD : ExprI.exprT tus tvs (typD u)) 
-    (Ha : exprD' tus tvs t a = Some aD) 
-    (Hb : exprD' tus tvs u b = Some bD)  :
-    exprD' tus tvs (tyProd t u) (mkPair t u a b) = Some (exprT_App (exprT_App (fun _ _ => pairD t u) aD) bD).
+        (aD : ExprI.exprT tus tvs (typD t)) 
+        (bD : ExprI.exprT tus tvs (typD u)) 
+        (Ha : exprD' tus tvs t a = Some aD) 
+        (Hb : exprD' tus tvs u b = Some bD)  :
+    exprD' tus tvs (tyProd t u) (mkPair t u a b) = 
+    Some (exprT_App (exprT_App (fun _ _ => pairD t u) aD) bD).
   Proof.
     unfold mkPair; simpl.
     autorewrite with exprD_rw; simpl; forward; inv_all; subst.
@@ -308,15 +315,15 @@ Section MakePairFuncSound.
     rewrite H1. unfold funcAs; simpl.
     rewrite type_cast_refl; [reflexivity | apply _].
   Qed.
-
+  
 End MakePairFuncSound.
 
 Section PairCases.
   Context {typ func : Type} {LF : PairFunc typ func}.
-
+  
   Definition pair_cases (e : expr typ func) (P : expr typ func -> Type)
-    (f_prod : forall t u f a b, pairS f = Some (pPair t u) -> P (App (App (Inj f) a) b))
-    (f_default : P e) : P e := 
+             (f_prod : forall t u f a b, pairS f = Some (pPair t u) -> P (App (App (Inj f) a) b))
+             (f_default : P e) : P e := 
     match e as e' return e = e' -> P e with
       | App (App (Inj f) a) b =>
         match pairS f as e'' return pairS f = e'' -> e = App (App (Inj f) a) b -> P e with
@@ -328,31 +335,8 @@ Section PairCases.
         end eq_refl
       | _ => fun _ => f_default
     end eq_refl.
-    
+  
 End PairCases.      
-
-Section TypeOfApply.
-  Context {typ : Type} {RType_typ : RType typ}.
-
-  Context {Typ2_tyArr : Typ2 _ Fun}.
-  Context {Typ2Ok_tyArr : Typ2Ok Typ2_tyArr}.
-
-  Lemma type_of_apply_Some t u v (H : type_of_apply t u = Some v) : t = typ2 u v.
-
-    unfold type_of_apply in H.
-    destruct (typ2_match_case t) as [[a [b [pf H1]]] | H1].
-    unfold Rty in pf. subst.
-    rewrite typ2_match_iota in H.
-    unfold eq_sym in H.
-    forward. apply _.
-    specialize (H1 (fun _ => option typ)).
-    specialize (H1 (fun d r => match type_cast d u with | Some _ => Some r | None => None end)).
-    simpl in H1. specialize (H1 None). rewrite H in H1. congruence.
-  Qed.
-
-End TypeOfApply.
-
-
 
 Section PairInversion.
   Context {typ func : Type} {PF : PairFunc typ func}.
@@ -423,11 +407,12 @@ Section PairInversion.
     assert (t4 = tyArr t0 (tyArr t1 (tyProd t0 t1)))  
       by (eapply pair_func_type_eq; eassumption).
     subst.
-    apply type_of_apply_Some in H2.
+
+    apply ExprFacts.type_of_apply_Some in H2.
     apply typ2_inj in H2; [|apply _].
     destruct H2.
     unfold Rty in *. subst.
-    apply type_of_apply_Some in HType.
+    apply ExprFacts.type_of_apply_Some in HType.
     apply typ2_inj in HType; [|apply _].
     destruct HType.
     apply typ2_inj in H3; [|apply _].
